Added receivefresh construct

aneris/examples/echo/echo_proof.v
@@ -1,9 +1,12 @@
+From aneris.aneris_lang.lib Require Import inject.
 From iris.algebra Require Import excl_auth.
 From trillium.prelude Require Import finitary.
+From aneris.prelude Require Import gset_map.
 From aneris.aneris_lang Require Import tactics proofmode adequacy.
 From aneris.aneris_lang.program_logic Require Import
      aneris_weakestpre aneris_adequacy aneris_lifting.
 From aneris.aneris_lang.lib Require Import network_util_proof assert_proof.
+From aneris.aneris_lang.lib Require Import list_code list_proof.
 From aneris.examples.echo Require Export echo_code.
 Set Default Proof Using "Type".
 
@@ -94,6 +97,82 @@ Section echo_client_proof.
   Definition clt_si γ : message → iProp Σ :=
     λ m, own_frag γ (m.(m_body)).
 
+  Definition receivefresh : val :=
+    λ: "skt" "ms",
+      letrec: "loop" <> :=
+      let: "msg" := unSOME (ReceiveFrom "skt") in
+      (if: list_mem "msg" "ms" then "loop" #() else "msg") in "loop" #().
+
+  Definition pair_to_msg (sa : socket_address)
+             (m : message_body * socket_address) : message :=
+    mkMessage m.2 sa IPPROTO_UDP m.1.
+
+  Instance pair_to_msg_injective sa : Inj eq eq (pair_to_msg sa).
+  Proof. intros [] [] Heq. by simplify_eq. Qed.
+
+  Lemma wp_receivefresh a φ R T h l (ms : list (message_body * socket_address)) :
+    is_list ms l →
+    R = gset_map (pair_to_msg a) (list_to_set ms) →
+    {{{ h ↪[ip_of_address a] (udp_socket (Some a) true) ∗
+        a ⤇ φ ∗ a ⤳ (R, T) }}}
+      receivefresh #(LitSocket h) l @[ip_of_address a]
+    {{{ m, RET (#(m_body m), #(m_sender m));
+        ⌜m_destination m = a⌝ ∗
+        h ↪[ip_of_address a] (udp_socket (Some a) true) ∗
+        a ⤳ ({[m]} ∪ R, T) ∗ φ m }}}.
+  Proof.
+    iIntros (Hl Heq Φ) "(Hh & #Hsi & Ha) HΦ".
+    wp_lam.
+    do 5 wp_pure _.
+    iLöb as "IH".
+    wp_pures.
+    wp_apply (aneris_wp_receivefrom with "[$Hh $Ha $Hsi]"); [try eauto..|].
+    iIntros (m) "[%Hdest H]".
+    wp_apply wp_unSOME; [done|]. iIntros "_".
+    wp_pures.
+    wp_apply (wp_list_mem _ ms l (m_body m, m_sender m)); [by iPureIntro|].
+    iDestruct "H" as "[H|H]".
+    - iDestruct "H" as "(%Hnin & Hh & Ha & _ & Hm)".
+      iIntros ([]) "%Hb".
+      { rewrite Heq in Hnin. 
+        (* Search list_to_set elem_of. *)
+        assert ((m_body m, m_sender m) ∈ (list_to_set ms: gset _)) as Hb'.
+        { by apply elem_of_list_to_set. }
+        apply (gset_map_correct1 (pair_to_msg a)) in Hb'.
+        assert (pair_to_msg a (m_body m, m_sender m) = m) as Heq'.
+        { destruct m. simplify_eq. done. }
+        rewrite Heq' in Hb'.
+        done. }
+      wp_pures. iApply "HΦ". by iFrame.
+    - iDestruct "H" as "(%Hin & Hh & Ha)".
+      iIntros ([]) "%Hb"; last first.
+      { destruct Hb as [Hb|Hb]; last first.
+        { rewrite Heq in Hin. rewrite Hb in Hin. set_solver. }
+        rewrite Heq in Hin.
+        assert ((m_body m, m_sender m) ∉ (list_to_set ms: gset _)) as Hb'.
+        { by apply not_elem_of_list_to_set. }
+        apply (gset_map_not_elem_of (pair_to_msg a)) in Hb'; [|apply _].
+        assert (pair_to_msg a (m_body m, m_sender m) = m) as Heq'.
+        { destruct m. simplify_eq. done. }
+        rewrite Heq' in Hb'.
+        done. }
+      wp_pure _.
+      iApply ("IH" with "Hh Ha HΦ").
+  Qed.
+
+  (* TODO: Remove when receivefresh has been ported *)
+  Definition echo_client : val := λ: "c_addr" "s_addr",
+    let: "socket" := NewSocket #PF_INET #SOCK_DGRAM #IPPROTO_UDP in
+    SocketBind "socket" "c_addr";;
+    SendTo "socket" #"Hello" "s_addr";;
+    let: "m1" := unSOME (ReceiveFrom "socket") in
+    SendTo "socket" #"World" "s_addr";;
+    let: "m2" := receivefresh "socket" ["m1"] in
+    let: "m1'" := Fst "m1" in
+    let: "m2'" := Fst "m2" in
+    assert: ("m1'" = #"Hello");;
+    assert: ("m2'" = #"World").
+
   Lemma echo_client_spec (sa srv_sa : socket_address) :
     {{{ unallocated {[sa]} ∗
         free_ports (ip_of_address sa) {[(port_of_address sa)]} ∗
@@ -134,25 +213,23 @@ Section echo_client_proof.
       iFrame "#∗". simpl. iIntros "!>" (m') "[%Hm Hm]". by rewrite Hm. }
     iIntros "[Hsh Hsa]".
     wp_pures.
-    wp_apply (aneris_wp_receivefrom with "[$Hsh $Hsa $Hsi]"); [try done..|].
+    wp_apply (wp_list_cons ((m_body m), (m_sender m)) []).
+    { iPureIntro. done. }
+    iIntros (v Hl).
+    wp_apply (wp_receivefresh with "[$Hsh $Hsa $Hsi]"); [done| |].
+    { simpl.
+      rewrite !union_empty_r_L.
+      rewrite gset_map_singleton.
+      rewrite /pair_to_msg.
+      f_equiv. simpl.
+      destruct m. 
+      simplify_eq. simpl.
+      destruct m_protocol.
+      done. }
     iIntros (m') "[%Hdst' H]".
-    wp_apply wp_unSOME; [done|]; iIntros "_".
-    iDestruct "H" as "[H|H]"; last first.
-    { iDestruct "H" as "[%Hin _]".
-      rewrite elem_of_union in Hin.
-      destruct Hin as [Hin|Hin]; [|set_solver].
-      rewrite elem_of_singleton in Hin.
-      simplify_eq.
-      wp_pures. case_bool_decide as Heql; [|by eauto].
-      wp_pures. by iApply "HΦ". }
-    wp_pures.
-    iDestruct "H" as "(%Hnin' & Hsh & Hsa & _ & Hfrag)".
+    iDestruct "H" as "(Hsh & Hsa & Hfrag)".
     iDestruct (own_valid_2 with "Hauth Hfrag") as %Hworld%excl_auth_agree_L.
-    case_bool_decide as Heq.
-    { assert (m = m') as ->.
-      { destruct m, m'. simplify_eq. simpl in *. simplify_eq. }
-      set_solver. }
-    do 7 wp_pure _.
+    do 8 wp_pure _.
     wp_apply wp_assert.
     wp_pures.
     iSplit; [iPureIntro; rewrite Hhello; case_bool_decide; done|].
@@ -168,7 +245,7 @@ End echo_client_proof.
 
 Definition echo_is :=
   {|
-    state_heaps :=  {["system" := ∅ ]};
+    state_heaps := {["system" := ∅ ]};
     state_sockets := {["system" := ∅ ]};
     state_ports_in_use := <["0.0.0.0" := ∅ ]> $ <["0.0.0.1" := ∅ ]> ∅;
     state_ms := ∅;
